Hoare2.v
@@ -1,0 +1,340 @@
+Add LoadPath "D:\sfsol".
+Require Export Hoare.
+
+Definition reduce_to_zero' : com :=
+  WHILE BNot (BEq (AId X) (ANum 0)) DO
+    X ::= AMinus (AId X) (ANum 1)
+  END.
+
+Theorem reduce_to_zero_correct' :
+  {{fun st => True}}
+  reduce_to_zero'
+  {{fun st => st X = 0}}.
+Proof.
+  unfold reduce_to_zero'.
+  (* First we need to transform the postcondition so
+     that hoare_while will apply. *)
+  eapply hoare_consequence_post.
+  apply hoare_while.
+  Case "Loop body preserves invariant".
+    (* Need to massage precondition before hoare_asgn applies *)
+    eapply hoare_consequence_pre. apply hoare_asgn.
+    (* Proving trivial implication (2) ->> (3) *)
+    intros st [HT Hbp]. unfold assn_sub. apply I.
+  Case "Invariant and negated guard imply postcondition".
+    intros st [Inv GuardFalse].
+    unfold bassn in GuardFalse. simpl in GuardFalse.
+    (* SearchAbout helps to find the right lemmas *)
+    SearchAbout [not true].
+    rewrite not_true_iff_false in GuardFalse.
+    SearchAbout [negb false].
+    rewrite negb_false_iff in GuardFalse.
+    SearchAbout [beq_nat true].
+    apply beq_nat_true in GuardFalse.
+    apply GuardFalse. Qed.
+
+Fixpoint parity x :=
+  match x with
+  | 0 => 0
+  | 1 => 1
+  | S (S x') => parity x'
+  end.
+
+Lemma parity_ge_2 : forall x,
+  2 <= x ->
+  parity (x - 2) = parity x.
+Proof.
+  intros. destruct x. inversion H. destruct x. inversion H. inversion H1.
+  simpl. rewrite <- minus_n_O. reflexivity.
+  Qed.
+
+Lemma parity_lt_2 : forall x,
+  ~ 2 <= x ->
+  parity (x) = x.
+Proof.
+  intros. destruct x; auto. destruct x; auto.
+  assert (False).
+  apply H. apply le_n_S. apply le_n_S. induction x;
+  constructor. auto. inversion H0.
+  Qed.
+
+Theorem parity_correct : forall m,
+    {{ fun st => st X = m }}
+  WHILE BLe (ANum 2) (AId X) DO
+    X ::= AMinus (AId X) (ANum 2)
+  END
+    {{ fun st => st X = parity m }}.
+Proof.
+  intros.
+  eapply hoare_consequence_post.
+    apply hoare_consequence_pre with (fun st => parity (st X) = parity m).
+      apply hoare_while.
+      eapply hoare_consequence_pre.
+        apply hoare_asgn.
+        intros st [H1 H2].
+        unfold assn_sub. simpl. rewrite update_eq.
+        rewrite parity_ge_2. assumption. 
+        apply ble_nat_true. apply H2.
+      intros st H; rewrite H; reflexivity.
+    intros st [H1 H2]. symmetry. rewrite <- parity_lt_2.
+      symmetry. assumption.
+      unfold not. intro. apply H2.
+      apply bexp_eval_true. simpl. destruct (st X); inversion H; auto.
+      destruct n. inversion H3. reflexivity.
+  Qed.
+
+Definition is_wp P c Q :=
+  {{P}} c {{Q}} /\
+  forall P', {{P'}} c {{Q}} -> (P' ->> P).
+
+Theorem is_wp_example :
+  is_wp (fun st => st Y <= 4)
+    (X ::= APlus (AId Y) (ANum 1)) (fun st => st X <= 5).
+Proof.
+  unfold is_wp.
+  split. eapply hoare_consequence_pre.
+  apply hoare_asgn. intros st H. unfold assn_sub.
+  rewrite update_eq. simpl. rewrite plus_comm.
+  apply le_n_S; auto.
+  intros. unfold hoare_triple in H.
+  intros st H1.
+  assert (update st X ((st Y) + 1 ) X <= 5).
+    eapply H.
+    constructor. auto. auto.
+  rewrite update_eq in H0. rewrite plus_comm in H0.
+  apply le_S_n. auto.
+  Qed.
+
+Theorem hoare_asgn_weakest : forall Q X a,
+  is_wp (Q [X |-> a]) (X ::= a) Q.
+Proof.
+  intros. unfold is_wp; split.
+  apply hoare_asgn.
+  unfold hoare_triple.
+  intros P H st H1.
+  assert(Q (update st X (aeval st a))).
+    eapply H; auto; try constructor; auto.
+  apply H0.
+  Qed.
+
+Module Himp.
+
+Inductive com : Type :=
+  | CSkip : com
+  | CAsgn : id -> aexp -> com
+  | CSeq : com -> com -> com
+  | CIf : bexp -> com -> com -> com
+  | CWhile : bexp -> com -> com
+  | CHavoc : id -> com.
+
+Tactic Notation "com_cases" tactic(first) ident(c) :=
+  first;
+  [ Case_aux c "SKIP" | Case_aux c "::=" | Case_aux c ";"
+  | Case_aux c "IFB" | Case_aux c "WHILE" | Case_aux c "HAVOC" ].
+
+Notation "'SKIP'" :=
+  CSkip.
+Notation "X '::=' a" :=
+  (CAsgn X a) (at level 60).
+Notation "c1 ;; c2" :=
+  (CSeq c1 c2) (at level 80, right associativity).
+Notation "'WHILE' b 'DO' c 'END'" :=
+  (CWhile b c) (at level 80, right associativity).
+Notation "'IFB' e1 'THEN' e2 'ELSE' e3 'FI'" :=
+  (CIf e1 e2 e3) (at level 80, right associativity).
+Notation "'HAVOC' X" := (CHavoc X) (at level 60).
+
+Reserved Notation "c1 '/' st '||' st'" (at level 40, st at level 39).
+
+Inductive ceval : com -> state -> state -> Prop :=
+  | E_Skip : forall st : state, SKIP / st || st
+  | E_Ass : forall (st : state) (a1 : aexp) (n : nat) (X : id),
+            aeval st a1 = n -> (X ::= a1) / st || update st X n
+  | E_Seq : forall (c1 c2 : com) (st st' st'' : state),
+            c1 / st || st' -> c2 / st' || st'' -> (c1 ;; c2) / st || st''
+  | E_IfTrue : forall (st st' : state) (b1 : bexp) (c1 c2 : com),
+               beval st b1 = true ->
+               c1 / st || st' -> (IFB b1 THEN c1 ELSE c2 FI) / st || st'
+  | E_IfFalse : forall (st st' : state) (b1 : bexp) (c1 c2 : com),
+                beval st b1 = false ->
+                c2 / st || st' -> (IFB b1 THEN c1 ELSE c2 FI) / st || st'
+  | E_WhileEnd : forall (b1 : bexp) (st : state) (c1 : com),
+                 beval st b1 = false -> (WHILE b1 DO c1 END) / st || st
+  | E_WhileLoop : forall (st st' st'' : state) (b1 : bexp) (c1 : com),
+                  beval st b1 = true ->
+                  c1 / st || st' ->
+                  (WHILE b1 DO c1 END) / st' || st'' ->
+                  (WHILE b1 DO c1 END) / st || st''
+  | E_Havoc : forall (st : state) (X : id) (n : nat),
+              (HAVOC X) / st || update st X n
+
+  where "c1 '/' st '||' st'" := (ceval c1 st st').
+
+Tactic Notation "ceval_cases" tactic(first) ident(c) :=
+  first;
+  [ Case_aux c "E_Skip" | Case_aux c "E_Ass" | Case_aux c "E_Seq"
+  | Case_aux c "E_IfTrue" | Case_aux c "E_IfFalse"
+  | Case_aux c "E_WhileEnd" | Case_aux c "E_WhileLoop"
+  | Case_aux c "E_Havoc" ].
+
+Definition hoare_triple (P:Assertion) (c:com) (Q:Assertion) : Prop :=
+  forall st st', c / st || st' -> P st -> Q st'.
+
+Notation "{{ P }}  c  {{ Q }}" := (hoare_triple P c Q) 
+                                  (at level 90, c at next level) 
+                                  : hoare_spec_scope.
+
+Definition havoc_pre (X : id) (Q : Assertion) : Assertion :=
+  fun st => forall n, Q[X|->ANum n] st.
+
+Theorem hoare_havoc : forall (Q : Assertion) (X : id),
+  {{ havoc_pre X Q }} HAVOC X {{ Q }}.
+Proof.
+  intros Q X st st' Heval Hpre.
+  inversion Heval; subst.
+  apply Hpre.
+  Qed.
+
+Lemma hoare_havoc_weakest : forall (P Q : Assertion) (X : id),
+  {{ P }} HAVOC X {{ Q }} ->
+  P ->> havoc_pre X Q.
+Proof.
+  intros P Q X H st H1.
+  unfold havoc_pre. intros n.
+  unfold hoare_triple in H.
+  assert(Q (update st X n)).
+    eapply H; try constructor; auto.
+  apply H0.
+  Qed.
+
+End Himp.
+
+Inductive dcom : Type :=
+  | DCSkip : Assertion -> dcom
+  | DCSeq : dcom -> dcom -> dcom
+  | DCAsgn : id -> aexp -> Assertion -> dcom
+  | DCIf : bexp -> Assertion -> dcom -> Assertion -> dcom
+           -> Assertion -> dcom
+  | DCWhile : bexp -> Assertion -> dcom -> Assertion -> dcom
+  | DCPre : Assertion -> dcom -> dcom
+  | DCPost : dcom -> Assertion -> dcom.
+
+Tactic Notation "dcom_cases" tactic(first) ident(c) :=
+  first;
+  [ Case_aux c "Skip" | Case_aux c "Seq" | Case_aux c "Asgn"
+  | Case_aux c "If" | Case_aux c "While"
+  | Case_aux c "Pre" | Case_aux c "Post" ].
+
+Notation "'SKIP' {{ P }}"
+      := (DCSkip P)
+      (at level 10) : dcom_scope.
+Notation "l '::=' a {{ P }}"
+      := (DCAsgn l a P)
+      (at level 60, a at next level) : dcom_scope.
+Notation "'WHILE' b 'DO' {{ Pbody }} d 'END' {{ Ppost }}"
+      := (DCWhile b Pbody d Ppost)
+      (at level 80, right associativity) : dcom_scope.
+Notation "'IFB' b 'THEN' {{ P }} d 'ELSE' {{ P' }} d' 'FI' {{ Q }}"
+      := (DCIf b P d P' d' Q)
+      (at level 80, right associativity) : dcom_scope.
+Notation "'->>' {{ P }} d"
+      := (DCPre P d)
+      (at level 90, right associativity) : dcom_scope.
+Notation "{{ P }} d"
+      := (DCPre P d)
+      (at level 90) : dcom_scope.
+Notation "d '->>' {{ P }}"
+      := (DCPost d P)
+      (at level 80, right associativity) : dcom_scope.
+Notation " d ;; d' "
+      := (DCSeq d d')
+      (at level 80, right associativity) : dcom_scope.
+
+Delimit Scope dcom_scope with dcom.
+
+Example dec_while : dcom := (
+  {{ fun st => True }}
+  WHILE (BNot (BEq (AId X) (ANum 0)))
+  DO
+    {{ fun st => True /\ st X <> 0}}
+    X ::= (AMinus (AId X) (ANum 1))
+    {{ fun _ => True }}
+  END
+  {{ fun st => True /\ st X = 0}} ->>
+  {{ fun st => st X = 0 }}
+) % dcom.
+
+Fixpoint extract (d:dcom) : com :=
+  match d with
+  | DCSkip _ => SKIP
+  | DCSeq d1 d2 => (extract d1 ;; extract d2)
+  | DCAsgn X a _ => X ::= a
+  | DCIf b _ d1 _ d2 _ => IFB b THEN extract d1 ELSE extract d2 FI
+  | DCWhile b _ d _ => WHILE b DO extract d END
+  | DCPre _ d => extract d
+  | DCPost d _ => extract d
+  end.
+
+Fixpoint post (d:dcom) : Assertion :=
+  match d with
+  | DCSkip P => P
+  | DCSeq d1 d2 => post d2
+  | DCAsgn X a Q => Q
+  | DCIf _ _ d1 _ d2 Q => Q
+  | DCWhile b Pbody c Ppost => Ppost
+  | DCPre _ d => post d
+  | DCPost c Q => Q
+  end.
+
+Fixpoint pre (d:dcom) : Assertion :=
+  match d with
+  | DCSkip P => fun st => True
+  | DCSeq c1 c2 => pre c1
+  | DCAsgn X a Q => fun st => True
+  | DCIf _ _ t _ e _ => fun st => True
+  | DCWhile b Pbody c Ppost => fun st => True
+  | DCPre P c => P
+  | DCPost c Q => pre c
+  end.
+
+Definition dec_correct (d:dcom) :=
+  {{pre d}} (extract d) {{post d}}.
+
+Fixpoint verification_conditions (P : Assertion) (d:dcom) : Prop :=
+  match d with
+  | DCSkip Q =>
+      (P ->> Q)
+  | DCSeq d1 d2 =>
+      verification_conditions P d1
+      /\ verification_conditions (post d1) d2
+  | DCAsgn l a Q =>
+      (P ->> Q [l |-> a])
+  | DCIf b P1 d1 P2 d2 Q =>
+      ((fun st => P st /\ bassn b st) ->> P1)
+      /\ ((fun st => P st /\ ~ (bassn b st)) ->> P2)
+      /\ (Q <<->> post d1) /\ (Q <<->> post d2)
+      /\ verification_conditions P1 d1
+      /\ verification_conditions P2 d2
+  | DCWhile b Pbody d Ppost =>
+      (P ->> post d)
+      /\ (Pbody <<->> (fun st => post d st /\ bassn b st))
+      /\ (Ppost <<->> (fun st => post d st /\ ~(bassn b st)))
+      /\ verification_conditions Pbody d
+  | DCPre P' d =>
+      (P ->> P') /\ verification_conditions P' d
+  | DCPost d Q =>
+      verification_conditions P d /\ (post d ->> Q)
+  end.
+
+Theorem verification_correct : forall d P,
+  verification_conditions P d -> {{P}} (extract d) {{post d}}.
+Proof.
+  induction d; intros P H; simpl in *.
+    eapply hoare_consequence_pre.
+      apply hoare_skip. assumption.
+    eapply hoare_seq;
+      inversion H as [H1 H2]. apply IHd2.
+      apply H2. apply IHd1. apply H1.
+    eapply hoare_consequence_pre.
+      apply hoare_asgn. assumption.
+    
